Huge update, with data from recovered files from Amazon machine.

Syntax.v.d
@@ -1,2 +1,0 @@
-Syntax.vo Syntax.glob Syntax.v.beautified: Syntax.v ../CompCert-3.0.1/lib/Coqlib.vo ../CompCert-3.0.1/lib/Integers.vo ./Expressions.vo ./Basics.vo ./AssertionSemantics.vo
-Syntax.vio: Syntax.v ../CompCert-3.0.1/lib/Coqlib.vio ../CompCert-3.0.1/lib/Integers.vio ./Expressions.vio ./Basics.vio ./AssertionSemantics.vio
